correctness/RegexCorrectness/VM/Path/VMPath.lean
@@ -55,14 +55,6 @@ end Regex.NFA
 namespace Regex.VM
 
 /--
-As an optimization, we write the updates to the buffer only when the state is done, a character, or a sparse state.
--/
-def WriteUpdate {nfa : NFA} (i : Fin nfa.nodes.size) : Prop :=
-  match nfa[i] with
-  | .done | .char _ _ | .sparse _ _ => True
-  | _ => False
-
-/--
 All states in `next.state` have a corresponding path from `nfa.start` to the state ending at `it`,
 and their updates are written to `next.updates` when necessary.
 -/
@@ -70,7 +62,7 @@ def SearchState.Inv (nfa : NFA) (wf : nfa.WellFormed) (it : Iterator) (next : Se
   ∀ i ∈ next.states,
     ∃ update,
       nfa.VMPath wf it i update ∧
-      (WriteUpdate i → next.updates[i] = update)
+      (εClosure.writeUpdate nfa[i] → next.updates[i] = update)
 
 theorem SearchState.Inv.of_empty {nfa wf it} {next : SearchState HistoryStrategy nfa} (h : next.states.isEmpty) :
   next.Inv nfa wf it := by
@@ -80,11 +72,7 @@ theorem SearchState.Inv.of_empty {nfa wf it} {next : SearchState HistoryStrategy
 end Regex.VM
 
 theorem Regex.NFA.CharStep.write_update {nfa : NFA} {it i j}
-  (step : nfa.CharStep it i j) : Regex.VM.WriteUpdate i := by
-  match hn : nfa[i] with
-  | .char c next => simp [hn, VM.WriteUpdate]
-  | .sparse cs next => simp [hn, VM.WriteUpdate]
-  | .done | .fail | .epsilon _ => simp_all
-  | .anchor _ _ => simp [anchor hn] at step
-  | .split _ _ => simp [split hn] at step
-  | .save _ _ => simp [save hn] at step
+  (step : nfa.CharStep it i j) : Regex.VM.εClosure.writeUpdate nfa[i] := by
+  match step.char_or_sparse with
+  | .inl ⟨c, next, eq⟩ => simp [Regex.VM.εClosure.writeUpdate, eq]
+  | .inr ⟨cs, next, eq⟩ => simp [Regex.VM.εClosure.writeUpdate, eq]
